Challenge/Bls12381/ProofSupport.lean
@@ -2,6 +2,7 @@ import Challenge.Bls12381.ProofSupport.Codec
 import Challenge.Bls12381.ProofSupport.Fp
 import Challenge.Bls12381.ProofSupport.FpRepresentation
 import Challenge.Bls12381.ProofSupport.FpConstants
+import Challenge.Bls12381.ProofSupport.FpWordBridge
 import Challenge.Bls12381.ProofSupport.FpAddSub
 import Challenge.Bls12381.ProofSupport.FpAddSubLawful
 import Challenge.Bls12381.ProofSupport.FpSchoolbook
